src/PlutusIR/Semantics/Dynamic/Values.v
@@ -26,40 +26,14 @@ Inductive value : term -> Prop :=
   | V_Constr : forall i T vs,
       Forall value vs ->
       value (Constr i T vs)
-  (** Unsaturated (partially applied) builtins *)
-  | V_Unsaturated : forall nv,
-      unsaturated_with 0 nv ->
-      value nv
-
-(* Applications of builtins that are unsaturated with n more arguments *)
-with unsaturated_with : nat -> term -> Prop :=
-  | U_Builtin : forall n f,
-      n < arity f ->
-      unsaturated_with n (Builtin f)
-  | U_Apply : forall n nv v,
-      value v ->
-      ~ is_error v ->
-      unsaturated_with (S n) nv ->
-      unsaturated_with n (Apply nv v)
-  | U_TyInst : forall n nv T,
-      unsaturated_with (S n) nv ->
-      unsaturated_with n (TyInst nv T)
   .
 
 #[export] Hint Constructors value : core.
-#[export] Hint Constructors unsaturated_with : core.
 
-Scheme value__ind := Minimality for value Sort Prop
-  with unsaturated_with__ind := Minimality for unsaturated_with Sort Prop.
-
-Combined Scheme value__multind from
-  value__ind,
-  unsaturated_with__ind.
-
-Section value_multind.
+Section value_ind.
 Context
   (P : term -> Prop)
-  (Q : nat -> term -> Prop).
+.
 Context
   (H_LamAbs : forall (x : String.string) (T : ty) (t0 : term), P (LamAbs x T t0))
   (H_TyAbs : forall (X : String.string) (K : kind) (t : term), P (TyAbs X K t))
@@ -67,99 +41,49 @@ Context
   (H_Constant : forall c : constant, P (Constant c))
   (H_Error : forall T : ty, P (Error T))
   (H_Constr : forall (i : nat) (T : ty) (vs : list term), Forall value vs -> Forall P vs -> P (Constr i T vs))
-  (H_unsaturated_with : forall nv : term, unsaturated_with 0 nv -> Q 0 nv -> P nv)
-  (H_Builtin : forall (n : nat) (f6 : DefaultFun), n < arity f6 -> Q n (Builtin f6))
-  (H_Apply : forall (n : nat) (nv v : term), value v -> P v -> ~ is_error v ->
-        unsaturated_with (S n) nv -> Q (S n) nv -> Q n (Apply nv v))
-  (H_TyInst : forall (n : nat) (nv : term) (T : ty),
-        unsaturated_with (S n) nv -> Q (S n) nv -> Q n (TyInst nv T)).
+.
 Fixpoint values__ind (H_value : forall (t : term), value t -> P t) (ts : list term) (vs : Forall value ts): Forall P ts :=
   match vs as vs in Forall _ ts return Forall P ts with
     | Forall_nil _ => Forall_nil _
     | @Forall_cons _ _ x xs vx vxs => @Forall_cons _ _ x xs (H_value x vx) (values__ind H_value xs vxs)
   end.
-Fixpoint value___ind (t : term) (v : value t) {struct v} : P t :=
+Fixpoint value__ind (t : term) (v : value t) {struct v} : P t :=
   match v in (value t0) return (P t0) with
   | V_LamAbs x T t0 => H_LamAbs x T t0
   | V_TyAbs X K t0 => H_TyAbs X K t0
-  | V_IWrap F1 T v0 v1 n => H_IWrap F1 T v0 v1 (value___ind v0 v1) n
+  | V_IWrap F1 T v0 v1 n => H_IWrap F1 T v0 v1 (value__ind v0 v1) n
   | V_Constant u => H_Constant u
   | V_Error T => H_Error T
   | V_Constr i T ts vs => H_Constr i T ts vs
       ((fix F ts vs := match vs as vs in Forall _ ts return Forall P ts with
         | Forall_nil _ => Forall_nil _
-        | @Forall_cons _ _ t ts vt vts => @Forall_cons _ _ t ts (value___ind t vt) (F ts vts)
+        | @Forall_cons _ _ t ts vt vts => @Forall_cons _ _ t ts (value__ind t vt) (F ts vts)
       end) ts vs)
-  | V_Unsaturated nv n => H_unsaturated_with nv n (unsaturated_with___ind 0 nv n)
-  end
-with unsaturated_with___ind (n : nat) (t : term) (n0 : unsaturated_with n t) {struct n0} : Q n t :=
-  match n0 in (unsaturated_with n1 t0) return (Q n1 t0) with
-  | U_Builtin n1 f9 l => H_Builtin n1 f9 l
-  | U_Apply n1 nv v v0 n2 n3 =>
-      H_Apply n1 nv v v0 (value___ind v v0) n2 n3 (unsaturated_with___ind (S n1) nv n3)
-  | U_TyInst n1 nv T n2 => H_TyInst n1 nv T n2 (unsaturated_with___ind (S n1) nv n2)
   end
 .
-Combined Scheme value___multind from value___ind, unsaturated_with___ind.
-End value_multind.
 
-Definition unsaturated (t : term) := unsaturated_with 0 t.
-
-#[export] Hint Unfold unsaturated : core.
-
-(* Applied builtin that is saturated with n more arguments *)
-Inductive saturated_with : nat -> term -> Prop :=
-  | S_Builtin : forall n f,
-      n = arity f ->
-      saturated_with n (Builtin f)
-  | S_Apply : forall n nv v,
+(* built-in that is applied to values/types of which the (type) arguments match
+   the signature *)
+Inductive applied_builtin : DefaultFun -> builtin_sig -> term -> Prop :=
+  | FA_Builtin : forall T f,
+      applied_builtin f (BS_Result T) (Builtin f)
+  | FA_Apply : forall f sig t v T,
       value v ->
       ~ is_error v ->
-      saturated_with (S n) nv ->
-      saturated_with n (Apply nv v)
-  | S_TyInst : forall n nv T,
-      saturated_with (S n) nv ->
-      saturated_with n (TyInst nv T)
+      applied_builtin f sig t ->
+      applied_builtin f (BS_Fun T sig) (Apply t v)
+  | FA_TyInst : forall f t T X K sig,
+      applied_builtin f sig t ->
+      applied_builtin f (BS_Forall X K sig) (TyInst t T)
   .
 
-#[export] Hint Constructors saturated_with : core.
+End value_ind.
 
-Definition saturated (t : term) := saturated_with 0 t.
-
-#[export] Hint Unfold saturated : core.
+(* A fully applied built-in is an applied_builtin for the corresponding
+   signature of that built-in *)
+Definition fully_applied t := exists f, applied_builtin f (to_sig f) t.
 
 Require Import Lia.
-
-Lemma unsaturated_with__monotone : forall n m nv,
-    unsaturated_with n nv ->
-    m <= n ->
-    unsaturated_with m nv.
-Proof with (eauto || (try lia)).
-  intros.
-  generalize dependent m.
-  induction H; intros...
-  - destruct f...
-    all: econstructor...
-  - econstructor...
-    eapply IHunsaturated_with...
-  - econstructor...
-    eapply IHunsaturated_with...
-Qed.
-
-Lemma saturated_with__subsumes__unsaturated_with : forall m n nv,
-  saturated_with n nv ->
-  m < n ->
-  unsaturated_with m nv.
-Proof with (eauto || (try lia)).
-  intros.
-  generalize dependent m.
-  induction H; intros...
-  - subst...
-  - econstructor...
-    eapply IHsaturated_with...
-  - econstructor...
-    eapply IHsaturated_with...
-Qed.
 
 
 Definition is_error_b (t : term) :=
@@ -206,5 +130,9 @@ Definition dec_unsaturated_with (n : nat) (t : term) :=
 Lemma dec_value_value : forall t, dec_value t = true -> value t.
 Admitted.
 
-Lemma dec_unsaturated_with_unsaturated_with : forall n t, dec_unsaturated_with n t = true -> unsaturated_with n t.
-Admitted.
+(* TODO: replace this by decision procedure for fully_applied *)
+Ltac not_fully_applied :=
+  inversion 1; 
+  repeat (match goal with H : applied_builtin _ _ _ |- _ => inversion H; clear H; subst end);
+  match goal with H : _ = to_sig _ |- _ => inversion H end
+.
