src/PlutusIR/Semantics/Dynamic/Bigstep/Deterministic.v
@@ -68,16 +68,8 @@ Ltac error_is_error :=
       exfalso; apply H; constructor
   end.
 
-Ltac invert_unsaturated :=
-  match goal with
-  | H : unsaturated ?t |- ?P =>
-      try solve [inversion H]
-  | H : unsaturated_with ?n ?t |- ?P =>
-      try solve [inversion H]
-  end.
-
 Ltac try_solve :=
-  try solve [repeat (use_IH || error_is_error || invert_unsaturated || eauto)].
+  try solve [repeat (use_IH || error_is_error || eauto)].
 
 (** ** The main result *)
 Theorem eval__deterministic : forall x y1 j1,
@@ -89,21 +81,6 @@ Proof with eauto.
   all: intros y5 j5 Hev.
   all: unfold_predicates.
   all: try solve [inversion Hev; subst; try_solve].
-  - inversion Hev; subst.
-    all: try_solve.
-    + inversion H10. subst.
-      apply eval_value in H12.
-      autounfold in H12.
-      use_IH.
-      inversion H10. subst.
-      inversion H15.
-    + inversion H8.
-      subst.
-      eapply saturated_with__subsumes__unsaturated_with in H13...
-      eapply eval_value in H13 as H14.
-      autounfold in H14.
-      use_IH.
-      invert_unsaturated.
 (* ADMIT: Remaining proof cases are technical overhead.
     Since we have multiple evaluation rules for applications
     and type instantiations, we need to do tedious work to
