src/PlutusIR/Semantics/Dynamic/Bigstep/EvalValue.v
@@ -5,10 +5,9 @@ Require Import PlutusCert.PlutusIR.Semantics.Dynamic.Bigstep.
 Require Import Lia.
 
 Lemma eval_value :
-  (forall v, value v -> v =[0]=> v) /\
-  (forall n v, unsaturated_with n v -> v =[0]=> v).
+  forall v, value v -> v =[0]=> v.
 Proof with (autounfold; (eauto || (try lia))).
-  apply value___multind.
+  apply value__ind.
   all: intros.
   all: try solve [constructor; eauto].
   (* Constr*)
@@ -16,25 +15,9 @@ Proof with (autounfold; (eauto || (try lia))).
     + constructor.
     + inversion H. inversion H0. subst.
       eapply E_Constr_cons with (k_t := 0) (k_ts := 0)...
-  - assumption.
-  - inversion H2; subst.
-    all: econstructor...
-    all: econstructor...
-    all: econstructor...
-    all: eapply unsaturated_with__monotone...
-  - inversion H; subst.
-    all: econstructor...
-    all: econstructor...
-    all: econstructor...
-    all: eapply unsaturated_with__monotone...
 Qed.
 
 Corollary eval_value__value : forall v,
     value v ->
     v =[0]=> v.
-Proof. apply eval_value. Qed.
-
-Corollary eval_value__neutral_value : forall n v,
-  unsaturated_with n v ->
-  v =[0]=> v.
 Proof. apply eval_value. Qed.
