src/PlutusIR/Semantics/Dynamic/Bigstep/Examples/IfThenElse.v
@@ -9,26 +9,8 @@ Require Import Coq.Strings.String.
 Local Open Scope string_scope.
 
 
-Ltac invert_neutrals :=
+Ltac decide_error :=
   match goal with
-  | H : unsaturated_with ?n ?t |- False =>
-      inversion H; clear H; subst; try invert_neutrals
-  | H : unsaturated ?t |- False =>
-      inversion H; clear H; subst; try invert_neutrals
-  end.
-
-Ltac decide_unsaturated :=
-  match goal with
-  | |- unsaturated ?nv =>
-      unfold unsaturated; econstructor; simpl; eauto; try decide_unsaturated
-  | |- unsaturated_with ?n ?nv =>
-      econstructor; simpl; eauto; try decide_unsaturated
-  | |- ?f <> ?f' =>
-      let Hcon := fresh "Hcon" in
-      try solve [intros Hcon; inversion Hcon]
-  | |- ~ unsaturated ?t =>
-      let Hcon := fresh "Hcon" in
-      try solve [intros Hcon; invert_neutrals]
   | |- ~ is_error ?t =>
       let Hcon := fresh "Hcon" in
       try solve [intros Hcon; inversion Hcon]
@@ -41,24 +23,35 @@ Definition int_and_int_to_int : ty := Ty_Fun Ty_int (Ty_Fun Ty_int Ty_int).
 
 Example test_ifThenElse : forall x y, exists k,
   <{
-    (λ x :: ℤ → ℤ → ℤ, {Var x} ⋅ Int 17 ⋅ Int 3)
-      ⋅ ((λ y :: ℤ, ifthenelse) ⋅ Int 666 @ ℤ ⋅ true)
+    (λ x :: ℤ → ℤ → ℤ, {Var x} ⋅ CInt 17 ⋅ CInt 3)
+      ⋅ ((λ y :: ℤ, ifthenelse) ⋅ CInt 666 @ ℤ ⋅ true)
   }>
-      =[k]=> <{ Int 17 }>.
-Proof with (eauto with hintdb__eval_no_error || (try solve [decide_unsaturated])).
-  unfold constInt.
+      =[k]=> <{ CInt 17 }>.
+Proof with (eauto with hintdb__eval_no_error || (try solve [decide_error])).
   intros.
   eexists.
   eapply E_Apply...
-  - eapply E_NeutralApplyPartial...
-    + eapply E_NeutralTyInstPartial...
+  - admit. (* TODO: decide fully_applied *)
+  - eapply E_Apply...
+    + admit.
+    + eapply E_TyInst...
+      * admit.
       * eapply E_Apply...
-      * simpl...
-      * eapply E_NeutralTyInst...
-    + simpl...
-    + eapply E_NeutralApply...
-  - simpl...
-  - simpl. rewrite eqb_refl.
-    eapply E_NeutralApplyFull...
-    repeat econstructor...
-Qed.
+        ** admit.
+        ** simpl.
+          eapply E_Builtin_Eta with (f := IfThenElse).
+      * constructor.
+    + cbn. constructor.
+  - inversion 1.
+  - cbn.
+    rewrite eqb_refl.
+    eapply E_Apply...
+    + admit.
+    + eapply E_Apply...
+      * admit.
+      * cbn.
+        constructor.
+    + cbn.
+      apply E_Builtin_Apply...
+      admit.
+Admitted.
